Review UInt and fix style

src/StandardLibrary/UInt.dfy
@@ -1,141 +1,141 @@
-module {:extern "STLUINT"} StandardLibrary.UInt {
-    newtype uint8 = x | 0 <= x < 256
+module {:extern "STLUInt"} StandardLibrary.UInt {
+  newtype UInt8 = x | 0 <= x < 256
 
-    newtype uint16 = x | 0 <= x < 0x1_0000
-    const UINT16_MAX := 0x1_0000 - 1
+  const UInt16_LIMIT := 0x1_0000
+  newtype UInt16 = x | 0 <= x < UInt16_LIMIT
 
-    newtype int32 = x | -0x8000_0000 <= x < 0x8000_0000
+  newtype Int32 = x | -0x8000_0000 <= x < 0x8000_0000
 
-    newtype uint32 = x | 0 <= x < 0x1_0000_0000
-    const UINT32_MAX := 0x1_0000_0000 - 1
+  const UInt32_LIMIT := 0x1_0000_0000
+  newtype UInt32 = x | 0 <= x < UInt32_LIMIT
 
-    newtype uint64 = x | 0 <= x < 0x1_0000_0000_0000_0000
+  newtype UInt64 = x | 0 <= x < 0x1_0000_0000_0000_0000
 
-    function method uint16ToSeq(x: uint16): seq<uint8>
-        ensures |uint16ToSeq(x)| == 2
-    {
-        var b0: uint8 := (x / 256) as uint8;
-        var b1: uint8 := (x % 256) as uint8;
-        [b0, b1]
-    }
+  function method UInt16ToSeq(x: UInt16): seq<UInt8>
+    ensures |UInt16ToSeq(x)| == 2
+  {
+    var b0: UInt8 := (x / 256) as UInt8;
+    var b1: UInt8 := (x % 256) as UInt8;
+    [b0, b1]
+  }
 
-    function method seqToUInt16(p: seq<uint8>): uint16 
-        requires |p| == 2
-    {
-        var x1 :=      (p[0] as int) * 256;
-        assert x1 <= 256 * 256;
-        var  x := x1 + (p[1] as int);
-        assert x <= UINT16_MAX;
-        x as uint16
-    }
+  function method SeqToUInt16(p: seq<UInt8>): UInt16
+    requires |p| == 2
+  {
+    var x1 :=    (p[0] as int) * 256;
+    assert x1 <= 256 * 256;
+    var  x := x1 + (p[1] as int);
+    assert x < UInt16_LIMIT;
+    x as UInt16
+  }
 
-    lemma uint16SeqSerDeser(x: uint16)
-        ensures seqToUInt16(uint16ToSeq(x)) == x
-    {}
+  lemma UInt16SeqSerDeser(x: UInt16)
+    ensures SeqToUInt16(UInt16ToSeq(x)) == x
+  {}
 
-    lemma uint16SeqDeserSer(s: seq<uint8>)
-        requires |s| == 2
-        ensures uint16ToSeq(seqToUInt16(s)) == s
-    {}
+  lemma UInt16SeqDeserSer(s: seq<UInt8>)
+    requires |s| == 2
+    ensures UInt16ToSeq(SeqToUInt16(s)) == s
+  {}
 
-    method uint16ToArray(x: uint16) returns (ret: array<uint8>)
-        ensures fresh(ret)
-        ensures uint16ToSeq(x) == ret[..]
-        ensures ret.Length == 2
-    {
-        ret := new uint8[2];
-        ret[0] := (x / 256) as uint8;
-        ret[1] := (x % 256) as uint8;
-    }
-    
-    function method arrayToUInt16(p: array<uint8>): (ret: uint16)
-        reads p
-        requires p.Length == 2
-        ensures seqToUInt16(p[..]) == ret
-    {
-        var x1 :=      p[0] as int * 256;
-        assert x1 <= 256 * 256;
-        var  x := x1 + p[1] as int;
-        assert x <= UINT16_MAX;
-        x as uint16
-    }
+  method UInt16ToArray(x: UInt16) returns (ret: array<UInt8>)
+    ensures fresh(ret)
+    ensures UInt16ToSeq(x) == ret[..]
+    ensures ret.Length == 2
+  {
+    ret := new UInt8[2];
+    ret[0] := (x / 256) as UInt8;
+    ret[1] := (x % 256) as UInt8;
+  }
 
-    function method uint32ToSeq(x: uint32): seq<uint8>
-        ensures |uint32ToSeq(x)| == 4
-    {
-        var b0 := ( x / 0x100_0000) as uint8;
-        var x0: uint32 :=  x - (b0 as uint32 * 0x100_0000);
+  function method arrayToUInt16(p: array<UInt8>): (ret: UInt16)
+    reads p
+    requires p.Length == 2
+    ensures SeqToUInt16(p[..]) == ret
+  {
+    var x1 :=    p[0] as int * 256;
+    assert x1 <= 256 * 256;
+    var  x := x1 + p[1] as int;
+    assert x < UInt16_LIMIT;
+    x as UInt16
+  }
 
-        var b1 := (x0 / 0x1_0000) as uint8;
-        var x1: uint32 := x0 - (b1 as uint32 * 0x1_0000);
+  function method UInt32ToSeq(x: UInt32): seq<UInt8>
+    ensures |UInt32ToSeq(x)| == 4
+  {
+    var b0 := ( x / 0x100_0000) as UInt8;
+    var x0: UInt32 :=  x - (b0 as UInt32 * 0x100_0000);
 
-        var b2 := (x1 / 0x100) as uint8;
-        // or for symmetry:
-        // x2 := x1 - (b2 * 0x100);
-        // b3 := (x2 / 1) as uint8;
-        var b3 := (x1 % 0x100) as uint8;
-        [b0, b1, b2, b3]
-    }
+    var b1 := (x0 / 0x1_0000) as UInt8;
+    var x1: UInt32 := x0 - (b1 as UInt32 * 0x1_0000);
 
-    function method seqToUInt32(p: seq<uint8>): uint32
-        requires |p| == 4
-    {
-        // 2^24 = 0x100_0000
-        var x3 :=      p[0] as int * 0x100_0000;
-        // 2^16 = 0x1_0000
-        var x2 := x3 + p[1] as int * 0x1_0000;
-        // 2^8 = 0x100
-        var x1 := x2 + p[2] as int * 0x100;
-        // 2^0 = 0x1
-        var  x := x1 + p[3] as int;
-        assert x <= UINT32_MAX;
-        x as uint32
-    }
+    var b2 := (x1 / 0x100) as UInt8;
+    // or for symmetry:
+    // x2 := x1 - (b2 * 0x100);
+    // b3 := (x2 / 1) as UInt8;
+    var b3 := (x1 % 0x100) as UInt8;
+    [b0, b1, b2, b3]
+  }
 
-    lemma uint32SeqSerDeser(x: uint32)
-        ensures seqToUInt32(uint32ToSeq(x)) == x
-    {}
+  function method SeqToUInt32(p: seq<UInt8>): UInt32
+    requires |p| == 4
+  {
+    // 2^24 = 0x100_0000
+    var x3 :=    p[0] as int * 0x100_0000;
+    // 2^16 = 0x1_0000
+    var x2 := x3 + p[1] as int * 0x1_0000;
+    // 2^8 = 0x100
+    var x1 := x2 + p[2] as int * 0x100;
+    // 2^0 = 0x1
+    var  x := x1 + p[3] as int;
+    assert x < UInt32_LIMIT;
+    x as UInt32
+  }
 
-    lemma uint32SeqDeserSer(s: seq<uint8>)
-        requires |s| == 4
-        ensures uint32ToSeq(seqToUInt32(s)) == s
-    {}
+  lemma UInt32SeqSerDeser(x: UInt32)
+    ensures SeqToUInt32(UInt32ToSeq(x)) == x
+  {}
 
-    method uint32ToArray(x: uint32) returns (ret: array<uint8>)
-        ensures fresh(ret)
-        ensures uint32ToSeq(x) == ret[..]
-        ensures ret.Length == 4
-    {
-        var x' := x;
-        ret := new uint8[4];
+  lemma UInt32SeqDeserSer(s: seq<UInt8>)
+    requires |s| == 4
+    ensures UInt32ToSeq(SeqToUInt32(s)) == s
+  {}
 
-        ret[0] := (x' / 0x100_0000) as uint8;
-        x' := x' - (ret[0] as uint32 * 0x100_0000);
+  method UInt32ToArray(x: UInt32) returns (ret: array<UInt8>)
+    ensures fresh(ret)
+    ensures UInt32ToSeq(x) == ret[..]
+    ensures ret.Length == 4
+  {
+    var x' := x;
+    ret := new UInt8[4];
 
-        ret[1] := (x' / 0x1_0000) as uint8;
-        x' := x' - (ret[1] as uint32 * 0x1_0000);
+    ret[0] := (x' / 0x100_0000) as UInt8;
+    x' := x' - (ret[0] as UInt32 * 0x100_0000);
 
-        ret[2] := (x' / 0x100) as uint8;
-        // or for symmetry:
-        // x' := x' - (ret[2] * 0x100);
-        // ret[3] := (x' / 1) as uint8;
-        ret[3] := (x' % 0x100) as uint8;
-    }
+    ret[1] := (x' / 0x1_0000) as UInt8;
+    x' := x' - (ret[1] as UInt32 * 0x1_0000);
 
-    function method arrayToUInt32(p: array<uint8>): (ret: uint32)
-        reads p
-        requires p.Length == 4
-        ensures seqToUInt32(p[..]) == ret
-    {
-        // 2^24 = 0x100_0000
-        var x3 :=      p[0] as int * 0x100_0000;
-        // 2^16 = 0x1_0000
-        var x2 := x3 + p[1] as int * 0x1_0000;
-        // 2^8 = 0x100
-        var x1 := x2 + p[2] as int * 0x100;
-        // 2^0 = 0x1
-        var  x := x1 + p[3] as int;
-        assert x <= UINT32_MAX;
-        x as uint32
-    }
+    ret[2] := (x' / 0x100) as UInt8;
+    // or for symmetry:
+    // x' := x' - (ret[2] * 0x100);
+    // ret[3] := (x' / 1) as UInt8;
+    ret[3] := (x' % 0x100) as UInt8;
+  }
+
+  function method ArrayToUInt32(p: array<UInt8>): (ret: UInt32)
+    reads p
+    requires p.Length == 4
+    ensures SeqToUInt32(p[..]) == ret
+  {
+    // 2^24 = 0x100_0000
+    var x3 :=    p[0] as int * 0x100_0000;
+    // 2^16 = 0x1_0000
+    var x2 := x3 + p[1] as int * 0x1_0000;
+    // 2^8 = 0x100
+    var x1 := x2 + p[2] as int * 0x100;
+    // 2^0 = 0x1
+    var  x := x1 + p[3] as int;
+    assert x < UInt32_LIMIT;
+    x as UInt32
+  }
 }
